Foundation/Vorspiel/BinaryRelations.lean
@@ -45,16 +45,12 @@ def Asymmetric := ∀ ⦃x y⦄, (x ≺ y) → ¬(y ≺ x)
 def Universal := ∀ ⦃x y⦄, x ≺ y
 class IsUniversal (α : Sort*) (r : α → α → Prop) : Prop where universal : Universal r
 
-abbrev ConverseWellFounded := WellFounded $ flip (· ≺ ·)
-class IsConverseWellFounded (α : Sort*) (r : α → α → Prop) : Prop where converse_well_founded : WellFounded $ flip r
-
 attribute [mk_iff]
   IsRefl
   IsSerial
   IsSymm
   IsTrans
   IsEuclidean
-  IsConverseWellFounded
   IsConfluent
   IsWeakConfluent
   IsConnected
@@ -152,100 +148,12 @@ lemma confluent_of_refl_connected (hRefl : Reflexive rel) (hConfl : Connected re
     . apply hRefl;
     . assumption;
 
-section ConverseWellFounded
-
-lemma ConverseWellFounded.iff_has_max : ConverseWellFounded r ↔ (∀ (s : Set α), Set.Nonempty s → ∃ m ∈ s, ∀ x ∈ s, ¬(r m x)) := by
-  simp [ConverseWellFounded, WellFounded.wellFounded_iff_has_min, flip]
-
-instance [Finite α] [IsTrans α rel] [IsIrrefl α rel] : IsConverseWellFounded _ rel := ⟨by
-  apply @Finite.wellFounded_of_trans_of_irrefl _ _ _
-    ⟨by intro a b c rba rcb; exact IsTrans.trans c b a rcb rba⟩
-    ⟨by simp [flip, IsIrrefl.irrefl]⟩
-⟩
-
-lemma Finite.converseWellFounded_of_trans_irrefl'
-    (hFinite : Finite α) (hTrans : Transitive rel) (hIrrefl : Irreflexive rel) : ConverseWellFounded rel :=
-  @Finite.wellFounded_of_trans_of_irrefl _ _ _
-    ⟨by simp [flip]; intro a b c ba cb; exact hTrans cb ba;⟩
-    ⟨by simp [flip]; exact hIrrefl⟩
-
-end ConverseWellFounded
-
-
+/-
 @[simp]
 lemma WellFounded.trivial_wellfounded : WellFounded (α := α) (λ _ _ => False) := by
   constructor; intro _;
   constructor; intro _ _;
   contradiction;
-
-def Relation.IrreflGen (R : α → α → Prop) := λ x y => x ≠ y ∧ R x y
-
-
-abbrev WeaklyConverseWellFounded (R : α → α → Prop) := ConverseWellFounded (Relation.IrreflGen R)
-alias WCWF := WeaklyConverseWellFounded
-
-
-section
-
-lemma dependent_choice {R : α → α → Prop} (h : ∃ s : Set α, s.Nonempty ∧ ∀ a ∈ s, ∃ b ∈ s, R a b)
-  : ∃ f : ℕ → α, ∀ x, R (f x) (f (x + 1)) := by
-  obtain ⟨s, ⟨x, hx⟩, h'⟩ := h;
-  choose! f hfs hR using h';
-  use fun n ↦ f^[n] x;
-  intro n;
-  simp only [Function.iterate_succ'];
-  refine hR (f^[n] x) ?a;
-  induction n with
-  | zero => simpa;
-  | succ n ih => simp only [Function.iterate_succ']; apply hfs _ ih;
-
-lemma Finite.exists_ne_map_eq_of_infinite_lt {α β} [LinearOrder α] [Infinite α] [Finite β] (f : α → β)
-  : ∃ x y : α, (x < y) ∧ f x = f y
-  := by
-    obtain ⟨i, j, hij, e⟩ := Finite.exists_ne_map_eq_of_infinite f;
-    rcases lt_trichotomy i j with (hij | _ | hij);
-    . use i, j;
-    . contradiction;
-    . use j, i; simp [hij, e];
-
-lemma antisymm_of_WCWF {R : α → α → Prop} : WCWF R → AntiSymmetric R := by
-  contrapose;
-  simp [AntiSymmetric];
-  intro x y Rxy Ryz hxy;
-  apply ConverseWellFounded.iff_has_max.not.mpr;
-  push_neg;
-  use {x, y};
-  constructor;
-  . simp;
-  . intro z hz;
-    by_cases z = x;
-    . use y; simp_all [Relation.IrreflGen];
-    . use x; simp_all [Relation.IrreflGen];
-
-lemma WCWF_of_finite_trans_antisymm {R : α → α → Prop} (hFin : Finite α) (R_trans : Transitive R)
-  : AntiSymmetric R → WCWF R := by
-    contrapose;
-    intro hWCWF;
-    replace hWCWF := ConverseWellFounded.iff_has_max.not.mp hWCWF;
-    push_neg at hWCWF;
-    obtain ⟨f, hf⟩ := dependent_choice hWCWF; clear hWCWF;
-    simp [Relation.IrreflGen] at hf;
-
-    simp [AntiSymmetric];
-    obtain ⟨i, j, hij, e⟩ := Finite.exists_ne_map_eq_of_infinite_lt f;
-    use (f i), (f (i + 1));
-    have ⟨hi₁, hi₂⟩ := hf i;
-    refine ⟨(by assumption), ?_, (by assumption)⟩;
-
-    have : i + 1 < j := lt_iff_le_and_ne.mpr ⟨by omega, by aesop⟩;
-    have H : ∀ i j, i < j → R (f i) (f j) := by
-      intro i j hij
-      induction hij with
-      | refl => exact hf i |>.2;
-      | step _ ih => exact R_trans ih $ hf _ |>.2;
-    have := H (i + 1) j this;
-    simpa [e];
-
-end
+-/
 
 end
