Foundation/Modal/Kripke/Basic.lean
@@ -48,13 +48,24 @@ def whitepoint : Frame := ⟨Unit, λ _ _ => True⟩
 instance : Finite whitepoint.World := by
   dsimp [whitepoint];
   infer_instance
-
+instance : IsRefl _ whitepoint.Rel := ⟨by tauto⟩
+instance : IsTrans _ whitepoint.Rel := ⟨by tauto⟩
+instance : IsEuclidean _ whitepoint.Rel := ⟨by tauto⟩
+instance : IsSymm _ whitepoint.Rel := ⟨by tauto⟩
+instance : IsSerial _ whitepoint.Rel := ⟨by tauto⟩
+instance : IsAntisymm _ whitepoint.Rel := ⟨by tauto⟩
+instance : IsPreorder _ whitepoint.Rel where
+instance : IsEquiv _ whitepoint.Rel where
+instance : IsPartialOrder _ whitepoint.Rel where
 
 def blackpoint : Frame := ⟨Unit, λ _ _ => False⟩
 
 instance : Finite blackpoint.World := by
   dsimp [blackpoint];
   infer_instance;
+instance : IsIrrefl _ blackpoint.Rel := by tauto
+instance : IsTrans _ blackpoint.Rel := ⟨by tauto⟩
+
 
 end
 
