Foundation/Modal/Kripke/Hilbert/S4Point3.lean
@@ -10,7 +10,7 @@ open Hilbert.Kripke
 open Geachean
 
 abbrev Kripke.FrameClass.connected_preorder : FrameClass := { F | IsPreorder _ F ∧ IsConnected _ F }
-abbrev Kripke.FrameClass.finite_connected_preorder : FrameClass := { F | F.IsFinite ∧ Reflexive F ∧ Transitive F ∧ Connected F }
+abbrev Kripke.FrameClass.finite_connected_preorder : FrameClass := { F | F.IsFinite ∧ IsPreorder _ F ∧ IsConnected _ F }
 
 /-
 namespace Kripke.FrameClass.connected_preorder
@@ -60,35 +60,36 @@ open
 instance finite_complete : Complete (Hilbert.S4Point3) Kripke.FrameClass.finite_connected_preorder := ⟨by
   intro φ hφ;
   apply Kripke.complete.complete;
-  rintro F ⟨F_refl, F_trans, F_conn⟩ V r;
+  rintro F ⟨_, _⟩ V r;
   let M : Kripke.Model := ⟨F, V⟩;
   let RM := M↾r;
-  have RM_refl : Reflexive RM.Rel := Frame.pointGenerate.rel_refl F_refl;
-  have RM_trans : Transitive RM.Rel := Frame.pointGenerate.rel_trans F_trans;
-
   apply Model.pointGenerate.modal_equivalent_at_root (M := M) (r := r) |>.mp;
 
   let FRM := finestFilterationTransitiveClosureModel RM (φ.subformulas);
-  apply filteration FRM (finestFilterationTransitiveClosureModel.filterOf RM_trans) (by aesop) |>.mpr;
+  apply filteration FRM (finestFilterationTransitiveClosureModel.filterOf (trans := Frame.pointGenerate.isTrans)) (by aesop) |>.mpr;
   apply hφ;
 
-  refine ⟨?_, ?_, ?_, ?_⟩;
+  refine ⟨?_, ?_, ?_⟩;
   . apply Frame.isFinite_iff _ |>.mpr
     apply FilterEqvQuotient.finite;
     simp;
-  . exact reflexive_of_transitive_reflexive RM_trans RM_refl;
-  . exact finestFilterationTransitiveClosureModel.transitive;
-  . rintro X ⟨y, (rfl | Rry)⟩ ⟨z, (rfl | Rrz)⟩ ⟨RXY, RXZ⟩;
-    . simp only [or_self]; apply Relation.TransGen.single; tauto;
-    . replace Rrz := TransGen.unwrap F_trans Rrz;
-      left;
-      apply Relation.TransGen.single $ by tauto;
-    . replace Rry := TransGen.unwrap F_trans Rry;
-      right;
-      apply Relation.TransGen.single $ by tauto;
-    . replace Rry := TransGen.unwrap F_trans Rry;
-      replace Rrz := TransGen.unwrap F_trans Rrz;
-      rcases F_conn ⟨Rry, Rrz⟩ with (Ryz | Rrw);
+  . exact finestFilterationTransitiveClosureModel.isPreorder (preorder := Frame.pointGenerate.isPreorder);
+  . apply isConnected_iff _ _ |>.mpr;
+    rintro X ⟨y, (rfl | Rry)⟩ ⟨z, (rfl | Rrz)⟩ ⟨RXY, RXZ⟩;
+    . simp only [or_self];
+      apply Relation.TransGen.single;
+      sorry;
+    . left;
+      apply Relation.TransGen.single;
+      replace Rrz := Rrz.unwrap;
+      tauto;
+    . right;
+      apply Relation.TransGen.single;
+      replace Rry := Rry.unwrap;
+      tauto;
+    . replace Rry := Rry.unwrap;
+      replace Rrz := Rrz.unwrap;
+      rcases IsConnected.connected ⟨Rry, Rrz⟩ with (Ryz | Rrw);
       . left; apply Relation.TransGen.single; tauto;
       . right; apply Relation.TransGen.single; tauto;
 ⟩
