Foundation/Vorspiel/Relation/Closure.lean
@@ -1,0 +1,25 @@
+import Mathlib.Logic.Relation
+
+namespace Relation
+
+variable {α} {r : α → α → Prop}
+
+
+namespace TransGen
+
+instance : IsTrans α (TransGen r) := ⟨by apply TransGen.trans⟩
+
+end TransGen
+
+
+
+section Irrefl
+
+def IrreflGen (r : α → α → Prop) := λ x y => x ≠ y ∧ r x y
+
+instance : IsIrrefl α (IrreflGen r) := ⟨by simp [IrreflGen]⟩
+
+end Irrefl
+
+
+end Relation
